Finished pushing through the list-Z-to-list-byte change (except that hkdf doesn't build for at least two other reasons)

hmacdrbg/HMAC256_DRBG_bridge_to_FCF.v
@@ -1,4 +1,5 @@
 Require Import hmacdrbg.spec_hmac_drbg.
+Require Import VST.floyd.functional_base.
 (*Require Import fcf.HMAC_DRBG_definitions_only.*)
 Require Import fcf.HMAC_DRBG_nonadaptive.
 Require Import sha.ByteBitRelations.
@@ -35,11 +36,11 @@ Proof.
   apply InBlocks_len; rewrite bytesToBits_len. exists (Datatypes.length l); omega.
 Qed.
 
-Lemma flatten_bytes_bits: forall m (M: Forall (Forall isbyteZ) m), 
+Lemma flatten_bytes_bits: forall m, 
       flatten m = bitsToBytes (flatten (map bytesToBits m)).
 Proof.
   induction m; simpl; trivial; intros.
-  inv M. rewrite IHm; clear IHm; trivial. 
+  rewrite IHm; clear IHm; trivial. 
   rewrite bitsToBytes_app, bytes_bits_bytes_id; trivial.
   apply bytesToBits_InBlocks. 
 Qed.
@@ -67,11 +68,10 @@ Proof. unfold HMAC_Blist, HMAC_Bvec. rewrite HMAC_equivalence.of_length_proof_ir
 Goal forall k' v, bitsToBytes (to_list (HMAC_Bvec k' v)) = HMAC256  (bitsToBytes v) (bitsToBytes (to_list k')).
 Proof. unfold HMAC_Bvec; intros.
   rewrite to_list_eq, HMAC_equivalence.of_length_proof_irrel, bytes_bits_bytes_id; trivial.
-  apply isbyteZ_HMAC256.
 Qed.
 
 Lemma HMAC_DRBG_generate_helper_Z_equation':
-  forall (HMAC : list Z -> list Z -> list Z) (key v : list Z) (requested_number_of_bytes : Z),
+  forall (HMAC : list byte -> list byte -> list byte) (key v : list byte) (requested_number_of_bytes : Z),
   0 < requested_number_of_bytes ->
   HMAC_DRBG_generate_helper_Z HMAC key v requested_number_of_bytes =
     let (v0, rest) := HMAC_DRBG_generate_helper_Z HMAC key v (requested_number_of_bytes - Z.of_nat 32) in
@@ -81,7 +81,7 @@ Proof. intros. rewrite HMAC_DRBG_generate_helper_Z_equation.
   symmetry in Heqb;  apply Z.geb_le in Heqb. omega.
 Qed. 
 Lemma HMAC_DRBG_generate_helper_Z_equation0:
-  forall (HMAC : list Z -> list Z -> list Z) (key v : list Z),
+  forall (HMAC : list byte -> list byte -> list byte) (key v : list byte),
   HMAC_DRBG_generate_helper_Z HMAC key v 0 = (v, nil).
 Proof. intros. rewrite HMAC_DRBG_generate_helper_Z_equation. trivial. Qed.
 
@@ -174,9 +174,9 @@ induction n; simpl; intros; subst.
   rewrite HMAC_Blist_Bvec, to_list_eq, list_append_map. split; trivial.
 Qed.
 
-(*Variant of Gen_loop_bvec that uses list Z instead of Bvector 256*)
-Fixpoint Gen_loop_Zlist (k : list Z) (v : list Z) (n : nat)
-  : list (list Z) * (list Z) :=
+(*Variant of Gen_loop_bvec that uses list byte instead of Bvector 256*)
+Fixpoint Gen_loop_Zlist (k : list byte) (v : list byte) (n : nat)
+  : list (list byte) * (list byte) :=
   match n with
   | O => (nil, v)
   | S n' =>
@@ -184,19 +184,6 @@ Fixpoint Gen_loop_Zlist (k : list Z) (v : list Z) (n : nat)
     let (bits, v'') := Gen_loop_Zlist k v' n' in
     (List.app bits (List.cons v' List.nil), v'')     
   end.
-
-Lemma Gen_loop_Zlist_isbyteZ k (K: Forall isbyteZ k): 
-  forall n v (V: Forall isbyteZ v),
-  match Gen_loop_Zlist k v n with (blocks,u) => 
-        Forall (Forall isbyteZ) blocks /\ Forall isbyteZ u 
-  end.
-Proof. induction n; simpl; intros.
-+ split; trivial.
-+ remember (Gen_loop_Zlist k (HMAC256 v k) n) as p; destruct p.
-  specialize (IHn (HMAC256 v k)). rewrite <- Heqp in IHn; destruct IHn. apply isbyteZ_HMAC256.
-  split; trivial. rewrite hmac_pure_lemmas.Forall_app. split; trivial.
-  constructor. apply isbyteZ_HMAC256. eauto.
-Qed. 
 
 Lemma Gen_loop_Zlist_ZlengthBlocks k: forall n v blocks u,
   Gen_loop_Zlist k v n = (blocks,u) -> Zlength blocks = Z.of_nat n.
@@ -208,8 +195,8 @@ Proof. induction n; intros.
   rewrite sublist.Zlength_app, Zlength_cons, (IHn _ _ (eq_refl _)). simpl; omega.
 Qed. 
 
-Lemma Gen_loop_Zlist_Blist k (K: Forall isbyteZ k):
-  forall n v (V: Forall isbyteZ v),
+Lemma Gen_loop_Zlist_Blist k:
+  forall n v,
   match Gen_loop_Zlist k v n with (blocks,u) =>
         Gen_loop_Blist (bytesToBits k) (bytesToBits v) n
         = (map bytesToBits blocks, bytesToBits u)
@@ -224,7 +211,7 @@ Proof. induction n; intros.
   destruct q. unfold HMAC_Blist in *.
   rewrite ! bytes_bits_bytes_id in *; trivial.
   rewrite IHn in Heqq; clear IHn. inv Heqq. f_equal.
-  rewrite map_app; trivial. apply isbyteZ_HMAC256.
+  rewrite map_app; trivial.
 Qed.
 
 Lemma Gen_loop_Zlist_nestedV k: forall n v blocks u blocks' u',
@@ -306,7 +293,7 @@ Qed.
 Lemma E_aux k: forall n v blocks u,
                Gen_loop_Zlist k (HMAC256 v k) n = (blocks, u) ->
       flatten (rev blocks) ++ HMAC256 u k =
-      HMAC256 (HMAC256 v k) k ++ flatten (rev (map (fun z : list Z => HMAC256 z k) blocks)).
+      HMAC256 (HMAC256 v k) k ++ flatten (rev (map (fun z : list byte => HMAC256 z k) blocks)).
 Proof. induction n; intros.
 + inv H; simpl. rewrite app_nil_r; trivial.
 + simpl in H.
@@ -401,11 +388,11 @@ Proof. unfold GenUpdate_original_Bvec, GenUpdate_original_Blist.
   rewrite ! HMAC_Blist_Bvec; trivial.
 Qed.
 
-Definition GenUpdate_original_Zlist (state : list Z * list Z) (n : nat) :
-  (list (list Z) * (list Z * list Z)) :=
+Definition GenUpdate_original_Zlist (state : list byte * list byte) (n : nat) :
+  (list (list byte) * (list byte * list byte)) :=
   match state with (k, v) =>
     match Gen_loop_Zlist k v n with (blocks, v') => 
-        let k' := HMAC256 (v' ++ [Z0]) k in
+        let k' := HMAC256 (v' ++ [Byte.zero]) k in
         let v'' := HMAC256 v' k' in (blocks, (k', v''))
     end
   end.
@@ -417,32 +404,20 @@ Proof. destruct state; simpl; intros.
   remember (Gen_loop_Zlist l l0 n) as p; destruct p; symmetry in Heqp.
   inv H. apply Gen_loop_Zlist_ZlengthBlocks in Heqp; rewrite Heqp; trivial.
 Qed.
- 
-Lemma GenUpdate_original_Zlist_isbyteZ k (K: Forall isbyteZ k) v (V: Forall isbyteZ v) n blocks state':
-  GenUpdate_original_Zlist (k,v) n = (blocks,state') -> 
-  Forall (Forall isbyteZ) blocks /\ Forall isbyteZ (fst state') /\ Forall isbyteZ (snd state').
-Proof. simpl.
-  remember (Gen_loop_Zlist k v n) as p; destruct p; symmetry in Heqp.
-  specialize (Gen_loop_Zlist_isbyteZ _ K n _ V); rewrite Heqp. intros [A B] C; inv C.
-  split; trivial. simpl. split; apply isbyteZ_HMAC256.
-Qed.
 
-Lemma GenUpdate_original_Zlist_Blist k v n
-  (K: Forall isbyteZ k) (V: Forall isbyteZ v):
+Lemma GenUpdate_original_Zlist_Blist k v n:
   match GenUpdate_original_Zlist (k,v) n with (blocks,(k',v')) =>
     GenUpdate_original_Blist (bytesToBits k, bytesToBits v) n =
          (map bytesToBits blocks,(bytesToBits k', bytesToBits v'))
   end.
 Proof. unfold GenUpdate_original_Zlist, GenUpdate_original_Blist. 
   remember (Gen_loop_Zlist k v n) as p; symmetry in Heqp. destruct p as [bits v'].
-  specialize (Gen_loop_Zlist_Blist _ K n _ V). rewrite Heqp; intros Q. simpl in Q. 
+  specialize (Gen_loop_Zlist_Blist k n v). rewrite Heqp; intros Q. simpl in Q. 
   remember (Gen_loop_Blist (bytesToBits k) (bytesToBits v) n) as q; destruct q.
-  assert (W: (l, b) =(@map (list Z) ByteBitRelations.Blist bytesToBits bits, bytesToBits v')) by (rewrite <- Q, Heqq; trivial). 
+  assert (W: (l, b) =(@map (list byte) ByteBitRelations.Blist bytesToBits bits, bytesToBits v')) by (rewrite <- Q, Heqq; trivial). 
   clear Q Heqq; inv W. f_equal. unfold HMAC_Blist.
-  assert (T: Forall (Forall isbyteZ) nil) by eauto.
-  specialize (Gen_loop_Zlist_isbyteZ _ K n _ V); rewrite Heqp. intros [? ?]. 
   rewrite ! bitsToBytes_app, ! bytes_bits_bytes_id; trivial.
-  f_equal. unfold zeroes. simpl. apply  isbyteZ_HMAC256. 
+  f_equal. unfold zeroes. simpl.
   apply bytesToBits_InBlocks. 
 Qed. 
 
@@ -472,7 +447,7 @@ Qed.
 Opaque FunGenerate.
 
 Lemma Generate_Blist_ok RI k v z n (Z: (z<=RI)%Z) l kk vv zz 
-    (K: Forall isbyteZ k) (V:Forall isbyteZ v) (N:(0<n)%nat):
+    (N:(0<n)%nat):
     FunGenerate RI (v, k, z) (Z.of_nat ((32 * n)%nat)) = generate_algorithm_success l (kk,vv, zz) ->
     exists y,
     GenUpdate_original_Blist (bytesToBits k, bytesToBits v) n = 
@@ -482,12 +457,12 @@ Proof.
   remember (GenUpdate_original_Zlist (k,v) n) as g. symmetry in Heqg; destruct g as [a [b c]].
   specialize (GenerateCorrect RI k v z n Z N). rewrite Heqg; intros HH1 HH2.
   rewrite HH1 in HH2. exists a. inv HH2. repeat split; trivial. 
-  specialize (GenUpdate_original_Zlist_Blist k v n K V).
+  specialize (GenUpdate_original_Zlist_Blist k v n).
   rewrite Heqg; intros HH; rewrite HH; trivial.
 Qed. 
 
-Lemma Generate_Bvec_ok' RI (k: list Z) v z n (Z: (z<=RI)%Z) l kk vv zz (N:(0<n)%nat)
-    (K: Forall isbyteZ k) (KL: Datatypes.length (bytesToBits k) = 256%nat) (V:Forall isbyteZ v) (VL:Datatypes.length (bytesToBits v) = 256%nat):
+Lemma Generate_Bvec_ok' RI (k: list byte) v z n (Z: (z<=RI)%Z) l kk vv zz (N:(0<n)%nat)
+    (KL: Datatypes.length (bytesToBits k) = 256%nat) (VL:Datatypes.length (bytesToBits v) = 256%nat):
     FunGenerate RI (v, k, z) (Z.of_nat ((32 * n)%nat)) = generate_algorithm_success l (kk,vv, zz) ->
     match GenUpdate_original_Bvec (of_list_length _ KL, of_list_length _ VL) n with (blocks, kv) =>
     zz=z+1 /\ 
@@ -499,7 +474,7 @@ Proof.
   remember (GenUpdate_original_Zlist (k,v) n) as g. symmetry in Heqg; destruct g as [a [b c]].
   specialize (GenerateCorrect RI k v z n Z N). rewrite Heqg; intros HH1 HH2.
   rewrite HH1 in HH2. inv HH2. 
-  specialize (GenUpdate_original_Zlist_Blist k v n K V).
+  specialize (GenUpdate_original_Zlist_Blist k v n).
   rewrite Heqg. intros HH.
   specialize (GenUpdate_original_Blist_Bvec (of_list_length (bytesToBits k) KL)
                 (of_list_length (bytesToBits v) VL) n); intros X. 
@@ -509,14 +484,14 @@ Proof.
   simpl in X. simpl in Heqw. rewrite Heqw in X; clear Heqw.
   destruct k0 as [w u]. rewrite ! HMAC_equivalence.of_length_proof_irrel in X.
   simpl in HH. rewrite HH in X; clear HH. inv X. split. trivial. simpl.
-  apply  GenUpdate_original_Zlist_isbyteZ in Heqg; trivial. destruct Heqg as [isbyteA [isbyteVV isbyteKK]].
   rewrite <- H1, <- H2, ! bytes_bits_bytes_id; trivial.
   repeat split; trivial.
-  rewrite <- map_rev. f_equal. apply flatten_bytes_bits. apply Forall_rev; trivial.
+  rewrite <- map_rev. f_equal. apply flatten_bytes_bits.
 Qed.
+
 Lemma Generate_Bvec_ok RI k v z n (Z: (z<=RI)%Z) (N:(0<n)%nat)
-              (K: Forall isbyteZ k) (KL: Datatypes.length (bytesToBits k) = 256%nat)
-              (V:Forall isbyteZ v) (VL:Datatypes.length (bytesToBits v) = 256%nat):
+              (KL: Datatypes.length (bytesToBits k) = 256%nat)
+              (VL:Datatypes.length (bytesToBits v) = 256%nat):
     match GenUpdate_original_Bvec (of_list_length _ KL, of_list_length _ VL) n with (blocks, (kk,vv)) =>
           FunGenerate RI (v, k, z) (Z.of_nat ((32 * n)%nat)) 
           = generate_algorithm_success (firstn (32 * n) (bitsToBytes (flatten (rev (map (@Vector.to_list _ 256) blocks)))))
@@ -525,7 +500,7 @@ Lemma Generate_Bvec_ok RI k v z n (Z: (z<=RI)%Z) (N:(0<n)%nat)
 Proof.
   remember (GenUpdate_original_Zlist (k,v) n) as g. symmetry in Heqg; destruct g as [a [b c]].
   specialize (GenerateCorrect RI k v z n Z N). rewrite Heqg; intros HH; rewrite HH.
-  specialize (GenUpdate_original_Zlist_Blist _ _ n K V); rewrite Heqg; intros.
+  specialize (GenUpdate_original_Zlist_Blist k v n); rewrite Heqg; intros.
   remember ( GenUpdate_original_Bvec
     (of_list_length (bytesToBits k) KL, of_list_length (bytesToBits v) VL) n) as p.
   destruct p as [blocks [kk vv]]; symmetry in Heqp. 
@@ -533,14 +508,13 @@ Proof.
                  (of_list_length (bytesToBits v) VL) n).
   simpl. simpl in Heqp. rewrite Heqp; clear Heqp. simpl in H.
   rewrite ! HMAC_equivalence.of_length_proof_irrel. rewrite H; clear H. intros. inv H.
-  apply  GenUpdate_original_Zlist_isbyteZ in Heqg; trivial. destruct Heqg as [isbyteA [isbyteVV isbyteKK]].
   f_equal.
-  - f_equal. rewrite <- map_rev. apply flatten_bytes_bits. apply Forall_rev; trivial. 
+  - f_equal. rewrite <- map_rev. apply flatten_bytes_bits.
   - rewrite ! bytes_bits_bytes_id; trivial.
 Qed.
 
 Lemma Generate_ok' RI k v z n (Z: (z<=RI)%Z) l kk vv zz (N:(0<n)%nat)
-    (K: Forall isbyteZ k) (KL: Datatypes.length (bytesToBits k) = 256%nat) (V:Forall isbyteZ v) (VL:Datatypes.length (bytesToBits v) = 256%nat):
+    (KL: Datatypes.length (bytesToBits k) = 256%nat) (VL:Datatypes.length (bytesToBits v) = 256%nat):
     FunGenerate RI (v, k, z) (Z.of_nat ((32 * n)%nat)) = generate_algorithm_success l (kk,vv, zz) ->
     match GenUpdate_original_core (of_list_length _ KL, of_list_length _ VL) n with (blocks, kv) =>
     zz=z+1 /\ 
@@ -549,7 +523,7 @@ Lemma Generate_ok' RI k v z n (Z: (z<=RI)%Z) l kk vv zz (N:(0<n)%nat)
           l = firstn (32 * n) (bitsToBytes (flatten (map (@Vector.to_list _ 256) blocks)))
     end.
 Proof. intros.
-  specialize (Generate_Bvec_ok' RI k v z n Z l kk vv zz N K KL V VL H); clear H; intros.
+  specialize (Generate_Bvec_ok' RI k v z n Z l kk vv zz N KL VL H); clear H; intros.
   remember (GenUpdate_original_Bvec
         (of_list_length (bytesToBits k) KL,
         of_list_length (bytesToBits v) VL) n) as p; symmetry in Heqp; destruct p as [blocks state]. 
@@ -558,9 +532,10 @@ Proof. intros.
                 of_list_length (bytesToBits v) VL) n). 
   rewrite Heqp; clear Heqp; intros Q; rewrite Q, map_rev; apply H.
 Qed.
+
 Lemma Generate_ok RI k v z n (Z: (z<=RI)%Z) (N:(0<n)%nat)
-              (K: Forall isbyteZ k) (KL: Datatypes.length (bytesToBits k) = 256%nat)
-              (V:Forall isbyteZ v) (VL:Datatypes.length (bytesToBits v) = 256%nat):
+              (KL: Datatypes.length (bytesToBits k) = 256%nat)
+              (VL:Datatypes.length (bytesToBits v) = 256%nat):
     match GenUpdate_original_core (of_list_length _ KL, of_list_length _ VL) n with (blocks, (kk,vv)) =>
           FunGenerate RI (v, k, z) (Z.of_nat ((32 * n)%nat)) 
           = generate_algorithm_success (firstn (32 * n) (bitsToBytes (flatten (map (@Vector.to_list _ 256) blocks))))
@@ -574,7 +549,7 @@ Proof.
   specialize (GenUpdate_original_Bvec_correct (of_list_length (bytesToBits k) KL,
          of_list_length (bytesToBits v) VL) n). rewrite Heqp. 
   intros Q; rewrite Q; clear Q.
-  specialize (Generate_Bvec_ok RI k v z n Z N K KL V VL). rewrite Heqp; clear Heqp.
+  specialize (Generate_Bvec_ok RI k v z n Z N KL VL). rewrite Heqp; clear Heqp.
   intros W; rewrite W, map_rev; trivial. 
 Qed.
 
@@ -628,7 +603,7 @@ Qed.
 Lemma Bridge_ok' s I (n:nat) bytes F ss (M: mbedtls_generate s I (32 * Z.of_nat n) = Some(bytes, ss, F)) (N:(0 < n)%nat):
   match I with HMAC256DRBGabs k v reseed_counter entropy_len prediction_resistance reseed_interval =>
   reseed_counter <= reseed_interval -> prediction_resistance = false ->
-  forall (K: Forall isbyteZ k) (KL: Datatypes.length (bytesToBits k) = 256%nat) (V:Forall isbyteZ v) (VL:Datatypes.length (bytesToBits v) = 256%nat),
+  forall (KL: Datatypes.length (bytesToBits k) = 256%nat) (VL:Datatypes.length (bytesToBits v) = 256%nat),
   match F with HMAC256DRBGabs KK VV rc _ _ _ =>
   s=ss /\ rc=reseed_counter+1 /\
     match GenUpdate_original_core (Blist.of_list_length _ KL, Blist.of_list_length _ VL) n with (blocks, kv) =>
@@ -641,10 +616,10 @@ Proof.
  specialize (Bridge' _ _ _ _ _ _ M); destruct I; intros.
  specialize (H H0 H1). destruct F. destruct H as [HH1 [HH2 HH3]].
  split; trivial. split; trivial.
- specialize (Generate_ok' reseed_interval key V reseed_counter n H0 bytes V1 key0 reseed_counter0).
+ specialize (Generate_ok' reseed_interval key V reseed_counter n H0 bytes V0 key0 reseed_counter0).
  rewrite Nat2Z.inj_mul. simpl. rewrite HH3.
  clear HH3 M.
- intros ZZ. specialize (ZZ N K KL V0 VL (eq_refl _)).
+ intros ZZ. specialize (ZZ N KL VL (eq_refl _)).
  remember (HMAC_DRBG_nonadaptive.Gen_loop HMAC_Bvec
            (Blist.of_list_length (bytesToBits key) KL)
            (Blist.of_list_length (bytesToBits V) VL) n) as q.
@@ -674,7 +649,7 @@ Qed.
 Lemma mbedtls_generate_Bridge s I (n:nat) bytes F ss (M: mbedtls_generate s I (32 * Z.of_nat n) = Some(bytes, ss, F)) (N:(0 < n)%nat):
   match I with HMAC256DRBGabs k v reseed_counter entropy_len prediction_resistance reseed_interval =>
   reseed_counter <= reseed_interval -> prediction_resistance = false ->
-  forall (K: Forall isbyteZ k) (KL: Datatypes.length (bytesToBits k) = 256%nat) (V:Forall isbyteZ v) (VL:Datatypes.length (bytesToBits v) = 256%nat),
+  forall (KL: Datatypes.length (bytesToBits k) = 256%nat) (VL:Datatypes.length (bytesToBits v) = 256%nat),
   match F with HMAC256DRBGabs KK VV rc _ _ _ =>
   s=ss /\ rc=reseed_counter+1 /\
     match GenUpdate_original_core (Blist.of_list_length _ KL, Blist.of_list_length _ VL) n with (blocks, kv) =>
@@ -685,7 +660,7 @@ Lemma mbedtls_generate_Bridge s I (n:nat) bytes F ss (M: mbedtls_generate s I (3
   end end.
 Proof.
  specialize (Bridge_ok' _ _ _ _ _ _ M N); destruct I; intros.
- specialize (H H0 H1 K KL V0 VL). destruct F. destruct H as [HH1 [HH2 HH3]].
+ specialize (H H0 H1 KL VL). destruct F. destruct H as [HH1 [HH2 HH3]].
  split; trivial. split; trivial.
  remember (GenUpdate_original_core
           (Blist.of_list_length (bytesToBits key) KL,
@@ -742,4 +717,4 @@ Proof.
   destruct kv as [k v]. prog_simp. apply comp_spec_ret; trivial. 
 Qed.*)
 (*Could now optionally FCF-relate GenUpdate_original_refactored to Generate, for 
-  relational spec relating bvectors to list Z,  using the above Gallina equalities*)*)
+  relational spec relating bvectors to list byte,  using the above Gallina equalities*)*)
