hmacdrbg/drbg_protocol_specs.v
@@ -18,8 +18,7 @@ Definition WF (I:hmac256drbgabs):=
          Zlength (hmac256drbgabs_value I) = 32 /\ 
          0 < hmac256drbgabs_entropy_len I <= 384 /\
          RI_range (hmac256drbgabs_reseed_interval I) /\
-         0 <= hmac256drbgabs_reseed_counter I < Int.max_signed /\
-         Forall isbyteZ (hmac256drbgabs_value I).
+         0 <= hmac256drbgabs_reseed_counter I < Int.max_signed.
 
 Definition REP sh gv (Info:md_info_state) (A:hmac256drbgabs) (v: val): mpred :=
   EX a:hmac256drbgstate, 
@@ -54,25 +53,25 @@ Definition seedbufREP sh gv (Info:md_info_state) (info:val) (A:hmac256drbgabs) (
 (*based on hmac_drbg_seed_inst256_spec*)
 Definition drbg_seed_inst256_spec_abs :=
   DECLARE _mbedtls_hmac_drbg_seed
-   WITH sh: share, dp:_, ctx: val, info:val, len: Z, data:val, Data: list Z,
+   WITH sh: share, dp:_, ctx: val, info:val, len: Z, data:val, Data: list byte,
         Info: md_info_state, s:ENTROPY.stream, rc:Z, pr_flag:bool, ri:Z,
         handle_ss: DRBG_functions.DRBG_state_handle * ENTROPY.stream, gv: globals
     PRE [_ctx OF tptr (Tstruct _mbedtls_hmac_drbg_context noattr),
          _md_info OF tptr (Tstruct _mbedtls_md_info_t noattr),
          _custom OF tptr tuchar, _len OF tuint ]
        PROP (writable_share sh; 
-                 len = Zlength Data /\ 0 <= len <=256 /\ Forall isbyteZ Data /\
+                 len = Zlength Data /\ 0 <= len <=256 /\
              instantiate_function_256 s pr_flag (contents_with_add data (Zlength Data) Data)
                = ENTROPY.success (fst handle_ss) (snd handle_ss))
        LOCAL (temp _ctx ctx; temp _md_info info;
               temp _len (Vint (Int.repr len)); temp _custom data; gvars gv)
        SEP (seedREP sh dp rc pr_flag ri gv Info info ctx; Stream s;
-            da_emp sh (tarray tuchar (Zlength Data)) (map Vint (map Int.repr Data)) data)
+            da_emp sh (tarray tuchar (Zlength Data)) (map Vubyte Data) data)
     POST [ tint ]
        EX ret_value:_,
        PROP ()
        LOCAL (temp ret_temp (Vint ret_value))
-       SEP (da_emp sh (tarray tuchar (Zlength Data)) (map Vint (map Int.repr Data)) data;
+       SEP (da_emp sh (tarray tuchar (Zlength Data)) (map Vubyte Data) data;
             if Int.eq ret_value (Int.repr (-20864))
             then seedREP sh dp rc pr_flag ri gv Info info ctx * Stream s                 
             else !!(ret_value = Int.zero) &&                  
@@ -84,7 +83,7 @@ Definition drbg_seed_inst256_spec_abs :=
 
 Definition drbg_seed_buf_abs_spec :=
   DECLARE _mbedtls_hmac_drbg_seed_buf
-   WITH sh: share, ctx: val, info:val, d_len: Z, data:val, Data: list Z,
+   WITH sh: share, ctx: val, info:val, d_len: Z, data:val, Data: list byte,
         I: hmac256drbgabs, Info:md_info_state,
         gv: globals
     PRE [_ctx OF tptr (Tstruct _mbedtls_hmac_drbg_context noattr),
@@ -92,21 +91,21 @@ Definition drbg_seed_buf_abs_spec :=
          _data OF tptr tuchar, _data_len OF tuint ]
        PROP (writable_share sh; 
                 d_len = Zlength Data \/ d_len=0;
-             0 <= d_len <= Int.max_unsigned; Forall isbyteZ Data)
+             0 <= d_len <= Int.max_unsigned)
        LOCAL (temp _ctx ctx; temp _md_info info;
               temp _data_len (Vint (Int.repr d_len)); temp _data data; gvars gv)
        SEP (seedbufREP sh gv Info info I ctx;
-            da_emp sh (tarray tuchar (Zlength Data)) (map Vint (map Int.repr Data)) data)
+            da_emp sh (tarray tuchar (Zlength Data)) (map Vubyte Data) data)
     POST [ tint ]
        EX ret_value:_,
        PROP ()
        LOCAL (temp ret_temp ret_value)
-       SEP (da_emp sh (tarray tuchar (Zlength Data)) (map Vint (map Int.repr Data)) data *
+       SEP (da_emp sh (tarray tuchar (Zlength Data)) (map Vubyte Data) data *
             if Val.eq ret_value (Vint (Int.repr (-20864)))
             then seedbufREP sh gv Info info I ctx
             else match I with HMAC256DRBGabs key V RC EL PR RI =>
-                 EX KEY:list Z, EX VAL:list Z, EX p:val, EX mds:mdstate,
-                 !!(hmacdrbg.HMAC256_DRBG_functional_prog.HMAC256_DRBG_update (contents_with_add data d_len Data) V (list_repeat 32 1) = (KEY, VAL))
+                 EX KEY:list byte, EX VAL:list byte, EX p:val, EX mds:mdstate,
+                 !!(hmacdrbg.HMAC256_DRBG_functional_prog.HMAC256_DRBG_update (contents_with_add data d_len Data) V (list_repeat 32 Byte.one) = (KEY, VAL))
                  && md_full Ews key mds * malloc_token Tsh (Tstruct _hmac_ctx_st noattr) p *
                  REP sh gv Info (HMAC256DRBGabs KEY VAL RC EL PR RI) ctx end).
 
@@ -152,40 +151,38 @@ Definition drbg_setReseedInterval_spec_abs :=
 
 Definition drbg_update_abs_spec :=
   DECLARE _mbedtls_hmac_drbg_update
-   WITH contents: list Z,
+   WITH contents: list byte,
         additional: val, sha: share, add_len: Z,
         ctx: val, shc: share, I: hmac256drbgabs,
         gv: globals
      PRE [ _ctx OF (tptr t_struct_hmac256drbg_context_st),
            _additional OF (tptr tuchar), _add_len OF tuint ]
        PROP (readable_share sha; writable_share shc; 0 <= add_len <= Int.max_unsigned;
-             add_len = Zlength contents \/ add_len = 0;
-             Forall isbyteZ contents)
+             add_len = Zlength contents \/ add_len = 0)
        LOCAL (temp _ctx ctx;
               temp _additional additional;
               temp _add_len (Vint (Int.repr add_len));
               gvars gv)
        SEP (AREP shc gv I ctx;
-            da_emp sha (tarray tuchar (Zlength contents)) (map Vint (map Int.repr contents)) additional)
+            da_emp sha (tarray tuchar (Zlength contents)) (map Vubyte contents) additional)
     POST [ tvoid ]
        PROP ()
        LOCAL ()
        SEP (AREP shc gv (hmac256drbgabs_hmac_drbg_update I (contents_with_add additional add_len contents)) ctx;
-            da_emp sha (tarray tuchar (Zlength contents)) (map Vint (map Int.repr contents)) additional).
+            da_emp sha (tarray tuchar (Zlength contents)) (map Vubyte contents) additional).
 
 Definition drbg_reseed_spec_abs :=
   DECLARE _mbedtls_hmac_drbg_reseed
-   WITH contents: list Z,
+   WITH contents: list byte,
         additional: val, sha: share, add_len: Z,
         ctx: val, shc: share, I: hmac256drbgabs,
         s: ENTROPY.stream, gv: globals
     PRE [ _ctx OF (tptr t_struct_hmac256drbg_context_st), _additional OF (tptr tuchar), _len OF tuint ]
        PROP (readable_share sha; writable_share shc; 0 <= add_len <= Int.max_unsigned;
              add_len = Zlength contents;
-             0 < hmac256drbgabs_entropy_len I + Zlength (contents_with_add additional add_len contents) < Int.modulus;         
-             Forall isbyteZ contents)
+             0 < hmac256drbgabs_entropy_len I + Zlength (contents_with_add additional add_len contents) < Int.modulus)
        LOCAL (temp _ctx ctx; temp _additional additional; temp _len (Vint (Int.repr add_len)); gvars gv)
-       SEP ( da_emp sha (tarray tuchar add_len) (map Vint (map Int.repr contents)) additional;
+       SEP ( da_emp sha (tarray tuchar add_len) (map Vubyte contents) additional;
               AREP shc gv I ctx; Stream s)
     POST [ tint ]
        EX rv:_,
@@ -193,7 +190,7 @@ Definition drbg_reseed_spec_abs :=
        LOCAL (temp ret_temp rv)
        SEP (if ((zlt 256 add_len) || (zlt 384 (hmac256drbgabs_entropy_len I + add_len)))%bool
   then (!!(rv = Vint (Int.neg (Int.repr 5))) &&
-       (da_emp sha (tarray tuchar add_len) (map Vint (map Int.repr contents)) additional *
+       (da_emp sha (tarray tuchar add_len) (map Vubyte contents) additional *
          AREP shc gv I ctx * Stream s))
   else (let F := mbedtls_HMAC256_DRBG_reseed_function s I (contents_with_add additional add_len contents)
         in !!(return_value_relate_result F rv)
@@ -201,34 +198,34 @@ Definition drbg_reseed_spec_abs :=
                   ENTROPY.success (V, K, rc, _, pr) _ => HMAC256DRBGabs K V rc (hmac256drbgabs_entropy_len I) pr
                                 (hmac256drbgabs_reseed_interval I) end*)
                      (hmac256drbgabs_reseed I s (contents_with_add additional add_len contents))) ctx *
-              da_emp sha (tarray tuchar add_len) (map Vint (map Int.repr contents)) additional *
+              da_emp sha (tarray tuchar add_len) (map Vubyte contents) additional *
               Stream (get_stream_result F))).
 
-Definition generate_absPOST ret_value contents additional sha add_len output sho out_len ctx shc I gv s :=
+Definition generate_absPOST ret_value (contents: list byte) additional sha add_len output sho out_len ctx shc I gv s :=
 if out_len >? 1024
 then (!!(ret_value = Vint (Int.neg (Int.repr 3))) &&
        (data_at_ sho (tarray tuchar out_len) output *
-         da_emp sha (tarray tuchar add_len) (map Vint (map Int.repr contents)) additional *
+         da_emp sha (tarray tuchar add_len) (map Vubyte contents) additional *
          AREP shc gv I ctx * Stream s))
 else
   if (add_len >? 256)
   then (!!(ret_value = Vint (Int.neg (Int.repr 5))) &&
        (data_at_ sho (tarray tuchar out_len) output *
-         da_emp sha (tarray tuchar add_len) (map Vint (map Int.repr contents)) additional *
+         da_emp sha (tarray tuchar add_len) (map Vubyte contents) additional *
          AREP shc gv I ctx * Stream s))
   else let F := (mbedtls_HMAC256_DRBG_generate_function s I out_len (contents_with_add additional add_len contents))
        in (!!(return_value_relate_result F ret_value)) &&
           (match F with
             | ENTROPY.error _ _ => (data_at_ sho (tarray tuchar out_len) output)
-            | ENTROPY.success (bytes, _) _ => (data_at sho (tarray tuchar out_len) (map Vint (map Int.repr bytes)) output)
+            | ENTROPY.success (bytes, _) _ => (data_at sho (tarray tuchar out_len) (map Vubyte bytes) output)
           end *
-          da_emp sha (tarray tuchar add_len) (map Vint (map Int.repr contents)) additional *
+          da_emp sha (tarray tuchar add_len) (map Vubyte contents) additional *
           Stream (get_stream_result F) *
           AREP shc gv (hmac256drbgabs_generate I s out_len (contents_with_add additional add_len contents)) ctx).
 
 Definition hmac_drbg_generate_abs_spec :=
   DECLARE _mbedtls_hmac_drbg_random_with_add
-   WITH contents: list Z,
+   WITH contents: list byte,
         additional: val, sha: share, add_len: Z,
         output: val, sho: share, out_len: Z,
         ctx: val, shc: share,
@@ -240,12 +237,11 @@ Definition hmac_drbg_generate_abs_spec :=
              0 <= add_len <= Int.max_unsigned;
              0 <= out_len <= Int.max_unsigned;
              add_len = Zlength contents;
-             hmac256drbgabs_entropy_len I + Zlength contents <= 384;
-             Forall isbyteZ contents)
+             hmac256drbgabs_entropy_len I + Zlength contents <= 384)
        LOCAL (temp _p_rng ctx; temp _output output; temp _out_len (Vint (Int.repr out_len)); 
               temp _additional additional; temp _add_len (Vint (Int.repr add_len)); gvars gv)
        SEP (data_at_ sho (tarray tuchar out_len) output;
-            da_emp sha (tarray tuchar add_len) (map Vint (map Int.repr contents)) additional;
+            da_emp sha (tarray tuchar add_len) (map Vubyte contents) additional;
             AREP shc gv I ctx; Stream s)
     POST [ tint ]
        EX ret_value:_,
@@ -269,7 +265,7 @@ Definition drbg_random_abs_spec :=
     POST [ tint ] 
        PROP () 
        LOCAL (temp ret_temp (Vint Int.zero))
-       SEP (data_at sho (tarray tuchar n) (map Vint (map Int.repr bytes)) output;
+       SEP (data_at sho (tarray tuchar n) (map Vubyte bytes) output;
             AREP shc gv F ctx; Stream ss).
 
 Definition drbg_random_abs_spec1 :=
@@ -291,5 +287,5 @@ Definition drbg_random_abs_spec1 :=
                                  (hmac256drbgabs_reseed_interval I)
                       end) 
        LOCAL (temp ret_temp (Vint Int.zero))
-       SEP (data_at sho (tarray tuchar n) (map Vint (map Int.repr bytes)) output;
+       SEP (data_at sho (tarray tuchar n) (map Vubyte bytes) output;
             AREP shc gv F ctx; Stream ss).
