hmacdrbg/spec_hmac_drbg_pure_lemmas.v
@@ -1,5 +1,6 @@
 Require Import compcert.lib.Coqlib.
 Require Import List. Import ListNotations.
+Require Import VST.floyd.functional_base.
 
 Require Import sha.general_lemmas.
 Require Import sha.HMAC256_functional_prog.
@@ -10,11 +11,8 @@ Require Import hmacdrbg.HMAC_DRBG_algorithms.
 Require Import hmacdrbg.HMAC256_DRBG_functional_prog.
 Require Import hmacdrbg.spec_hmac_drbg.
 
-Lemma isbyteZ_initialKey: Forall isbyteZ initial_key.
-Proof. apply sublist.Forall_list_repeat; split; omega. Qed.
-
 Lemma hmac256drbgabs_hmac_drbg_update_any_prop_key:
-  forall (P: list Z -> Prop) a additional_data,
+  forall (P: list byte -> Prop) a additional_data,
     (forall x y, P (HMAC256 x y)) ->
     P (hmac256drbgabs_key (hmac256drbgabs_hmac_drbg_update a additional_data)).
 Proof.
@@ -25,7 +23,7 @@ Proof.
 Qed.
 
 Lemma hmac256drbgabs_hmac_drbg_update_any_prop_V:
-  forall (P: list Z -> Prop) a additional_data,
+  forall (P: list byte -> Prop) a additional_data,
     (forall x y, P (HMAC256 x y)) ->
     P (hmac256drbgabs_value (hmac256drbgabs_hmac_drbg_update a additional_data)).
 Proof.
@@ -53,26 +51,8 @@ Proof.
   apply hmac_common_lemmas.HMAC_Zlength.
 Qed.
 
-Lemma hmac256drbgabs_hmac_drbg_update_isbyteZ_key:
-  forall a additional_data,
-    Forall isbyteZ (hmac256drbgabs_key (hmac256drbgabs_hmac_drbg_update a additional_data)).
-Proof.
-  intros.
-  apply hmac256drbgabs_hmac_drbg_update_any_prop_key.
-  apply hmac_common_lemmas.isbyte_hmac.
-Qed.
-
-Lemma hmac256drbgabs_hmac_drbg_update_isbyteZ_V:
-  forall a additional_data,
-    Forall isbyteZ (hmac256drbgabs_value (hmac256drbgabs_hmac_drbg_update a additional_data)).
-Proof.
-  intros.
-  apply hmac256drbgabs_hmac_drbg_update_any_prop_V.
-  apply hmac_common_lemmas.isbyte_hmac.
-Qed.
-
 Lemma hmac256drbgabs_reseed_any_prop_key:
-  forall (P: list Z -> Prop) a s additional_data,
+  forall (P: list byte -> Prop) a s additional_data,
     P (hmac256drbgabs_key a) ->
     (forall x y, P (HMAC256 x y)) ->
     P (hmac256drbgabs_key (hmac256drbgabs_reseed a s additional_data)).
@@ -88,7 +68,7 @@ Proof.
 Qed.
 
 Lemma hmac256drbgabs_reseed_any_prop_V:
-  forall (P: list Z -> Prop) a s additional_data,
+  forall (P: list byte -> Prop) a s additional_data,
     P (hmac256drbgabs_value a) ->
     (forall x y, P (HMAC256 x y)) ->
     P (hmac256drbgabs_value (hmac256drbgabs_reseed a s additional_data)).
@@ -123,26 +103,6 @@ Proof.
   apply hmac_common_lemmas.HMAC_Zlength.
 Qed.
 
-Lemma hmac256drbgabs_reseed_isbyteZ_key:
-  forall a s additional_data,
-    Forall isbyteZ (hmac256drbgabs_key a) ->
-    Forall isbyteZ (hmac256drbgabs_key (hmac256drbgabs_reseed a s additional_data)).
-Proof.
-  intros.
-  apply hmac256drbgabs_reseed_any_prop_key; auto.
-  apply hmac_common_lemmas.isbyte_hmac.
-Qed.
-
-Lemma hmac256drbgabs_reseed_isbyteZ_V:
-  forall a s additional_data,
-    Forall isbyteZ (hmac256drbgabs_value a) ->
-    Forall isbyteZ (hmac256drbgabs_value (hmac256drbgabs_reseed a s additional_data)).
-Proof.
-  intros.
-  apply hmac256drbgabs_reseed_any_prop_V; auto.
-  apply hmac_common_lemmas.isbyte_hmac.
-Qed.
-
 Lemma hmac256drbgabs_update_key_ident:
   forall a key, key = hmac256drbgabs_key a -> hmac256drbgabs_update_key a key = a.
 Proof.
@@ -168,18 +128,12 @@ Proof.
   reflexivity.
 Qed.
 
-Lemma isbyteZ_HMAC256 V K: Forall isbyteZ (HMAC256 V K).
-Proof. apply hmac_common_lemmas.isbyte_hmac. Qed.
-
 Lemma HMAC_DRBG_update_value l key V key' V'
   (P:(key', V') = HMAC_DRBG_update HMAC256 l key V):
-  Zlength V' = 32 /\ Forall isbyteZ V'.
+  Zlength V' = 32.
 Proof. unfold HMAC_DRBG_update in P.
-  destruct l; inv P; split.
+  destruct l; inv P;
   apply hmac_common_lemmas.HMAC_Zlength.
-  apply isbyteZ_HMAC256.
-  apply hmac_common_lemmas.HMAC_Zlength.
-  apply isbyteZ_HMAC256.
 Qed.
 
 Lemma Zlength_hmac256drbgabs_reseed_value abs s c
@@ -198,31 +152,8 @@ Proof. unfold hmac256drbgabs_reseed. destruct abs.
     destruct q; inv H0. eapply HMAC_DRBG_update_value; eassumption.
 Qed.
 
-Lemma isbyteZ_hmac256drbgabs_reseed_value abs s c
-  (HC: Zlength c >? 256 = false) (HV: Forall isbyteZ (hmac256drbgabs_value abs)):
-  Forall isbyteZ (hmac256drbgabs_value (hmac256drbgabs_reseed abs s c)).
-Proof. unfold hmac256drbgabs_reseed. destruct abs.
-  remember (mbedtls_HMAC256_DRBG_reseed_function s
-         (HMAC256DRBGabs key V reseed_counter entropy_len
-            prediction_resistance reseed_interval) c) as d.
-  destruct d; trivial.
-  destruct d as [[[[? ?] ?] ?] ?]; simpl.
-    unfold mbedtls_HMAC256_DRBG_reseed_function, HMAC256_DRBG_reseed_function, DRBG_reseed_function in Heqd.
-    rewrite andb_negb_r, HC in Heqd.
-    destruct (get_entropy 32(*256*) entropy_len entropy_len prediction_resistance s); inv Heqd.
-    remember (HMAC_DRBG_update HMAC256 (l1 ++ c) key V) as q.
-    destruct q; inv H0. eapply HMAC_DRBG_update_value; eassumption.
-Qed.
-
 Lemma Zlength_hmac256drbgabs_update_value abs c:
   Zlength (hmac256drbgabs_value (hmac256drbgabs_hmac_drbg_update abs c)) = 32.
-Proof. unfold hmac256drbgabs_hmac_drbg_update. destruct abs.
-  remember (HMAC256_DRBG_update c key V) as d.
-  destruct d; simpl. eapply HMAC_DRBG_update_value; eassumption.
-Qed.
-
-Lemma isbyteZ_hmac256drbgabs_update_value abs c:
-  Forall isbyteZ (hmac256drbgabs_value (hmac256drbgabs_hmac_drbg_update abs c)).
 Proof. unfold hmac256drbgabs_hmac_drbg_update. destruct abs.
   remember (HMAC256_DRBG_update c key V) as d.
   destruct d; simpl. eapply HMAC_DRBG_update_value; eassumption.
